feat: add the named list of trait parameters in instances

lib/src/top_level.rs
@@ -114,14 +114,21 @@ enum TopLevelItem {
     },
     TraitImpl {
         generic_tys: Vec<String>,
-        // The boolean is there to indicate if the type parameter has a default
-        ty_params: Vec<(Box<CoqType>, bool)>,
+        /// The boolean is there to indicate if the type parameter has a default
+        ty_params: Vec<Box<TraitImplTyParam>>,
         self_ty: Box<CoqType>,
         of_trait: Path,
         items: Vec<(String, ImplItem)>,
         trait_non_default_items: Vec<String>,
     },
     Error(String),
+}
+
+#[derive(Debug)]
+struct TraitImplTyParam {
+    name: String,
+    ty: Box<CoqType>,
+    has_default: bool,
 }
 
 #[derive(Debug)]
@@ -524,19 +531,19 @@ fn compile_top_level_item(tcx: &TyCtxt, env: &mut Env, item: &Item) -> Vec<TopLe
                     let generics = tcx.generics_of(trait_ref.trait_def_id().unwrap());
 
                     // Get the list of type parameters default status (true if it has a default)
-                    let mut type_params_default_status: Vec<bool> = generics
+                    let mut type_params_name_and_default_status: Vec<(String, bool)> = generics
                         .params
                         .iter()
                         .filter_map(|param| match param.kind {
                             rustc_middle::ty::GenericParamDefKind::Type { has_default, .. } => {
-                                Some(has_default)
+                                Some((param.name.to_string(), has_default))
                             }
                             _ => None,
                         })
                         .collect();
                     // The first type parameter is always the Self type, that we do not consider as
                     // part of the list of type parameters.
-                    type_params_default_status.remove(0);
+                    type_params_name_and_default_status.remove(0);
 
                     let ty_params = compile_path_ty_params(env, trait_ref.path);
 
@@ -544,7 +551,14 @@ fn compile_top_level_item(tcx: &TyCtxt, env: &mut Env, item: &Item) -> Vec<TopLe
                         generic_tys,
                         ty_params: ty_params
                             .into_iter()
-                            .zip(type_params_default_status)
+                            .zip(type_params_name_and_default_status)
+                            .map(|(ty, (name, has_default))| {
+                                Box::new(TraitImplTyParam {
+                                    name,
+                                    ty,
+                                    has_default,
+                                })
+                            })
                             .collect(),
                         self_ty,
                         of_trait: compile_path(env, trait_ref.path),
@@ -1682,48 +1696,51 @@ impl TopLevelItem {
                         })),
                         nest([
                             nest([
-                                nest([text("Global Instance"), line(), text("I")]),
-                                text(" :"),
+                                text("Global Instance I :"),
                                 line(),
-                                nest([of_trait.to_doc(), text(".Trait"), line(), text("Self")]),
-                                concat(
-                                    generic_tys
-                                        .iter()
-                                        .map(text)
-                                        .zip(ty_params.iter().map(|(ty_param, has_default)| {
-                                            if *has_default {
-                                                nest([
-                                                    text("(Some"),
-                                                    line(),
-                                                    ty_param.to_doc(false),
-                                                    text(")"),
-                                                ])
-                                            } else {
-                                                ty_param.to_doc(false)
-                                            }
-                                        }))
-                                        .map(|(generic_ty_doc, ty_param_doc)| {
-                                            concat([
+                                nest([
+                                    of_trait.to_doc(),
+                                    text(".Trait"),
+                                    line(),
+                                    text("Self"),
+                                    concat(ty_params.iter().map(|ty_param| {
+                                        concat([
+                                            line(),
+                                            nest([
+                                                text("("),
+                                                text(ty_param.name.clone()),
                                                 line(),
-                                                nest([
-                                                    text("("),
-                                                    generic_ty_doc,
-                                                    line(),
-                                                    text(":"),
-                                                    line(),
-                                                    ty_param_doc,
-                                                    text(")"),
-                                                ]),
-                                            ])
-                                        }),
-                                ),
+                                                text(":="),
+                                                line(),
+                                                if ty_param.has_default {
+                                                    nest([
+                                                        text("(Some"),
+                                                        line(),
+                                                        ty_param.ty.to_doc(false),
+                                                        text(")"),
+                                                    ])
+                                                } else {
+                                                    ty_param.ty.to_doc(false)
+                                                },
+                                                text(")"),
+                                            ]),
+                                        ])
+                                    })),
+                                ]),
                             ]),
                             text(" :="),
-                            line(),
                             if items.is_empty() {
-                                nest([of_trait.to_doc(), text(".Build_Trait"), line(), text("_")])
+                                concat([
+                                    line(),
+                                    nest([
+                                        of_trait.to_doc(),
+                                        text(".Build_Trait"),
+                                        line(),
+                                        text("_"),
+                                    ]),
+                                ])
                             } else {
-                                text("{")
+                                text(" {")
                             },
                         ]),
                         nest(trait_non_default_items.iter().map(|name| {
