coq_translation/examples/error_handling/wrapping_errors.v
@@ -99,7 +99,8 @@ Module Impl_core_convert_From_for_wrapping_errors_DoubleError.
     Notation.double_colon := from;
   }.
   
-  Global Instance I : core.convert.From.Trait Self := {
+  Global Instance I :
+      core.convert.From.Trait Self (T := core.num.error.ParseIntError) := {
     core.convert.From.from := from;
   }.
 End Impl_core_convert_From_for_wrapping_errors_DoubleError.
