coq_translation/examples/generics/generics_associated_types_problem.v
@@ -60,7 +60,11 @@ Module
     Notation.dot := last;
   }.
   
-  Global Instance I : generics_associated_types_problem.Contains.Trait Self := {
+  Global Instance I :
+      generics_associated_types_problem.Contains.Trait
+        Self
+        (A := i32)
+        (B := i32) := {
     generics_associated_types_problem.Contains.contains := contains;
     generics_associated_types_problem.Contains.first := first;
     generics_associated_types_problem.Contains.last := last;
