coq_translation/examples/traits/disambiguating_overlapping_traits.v
@@ -48,8 +48,7 @@ Module
   }.
   
   Global Instance I :
-      disambiguating_overlapping_traits.UsernameWidget.Trait Self :=
-    {
+      disambiguating_overlapping_traits.UsernameWidget.Trait Self := {
     disambiguating_overlapping_traits.UsernameWidget.get := get;
   }.
 End
@@ -65,8 +64,8 @@ Module
     Notation.dot := get;
   }.
   
-  Global Instance I : disambiguating_overlapping_traits.AgeWidget.Trait Self :=
-    {
+  Global Instance I :
+      disambiguating_overlapping_traits.AgeWidget.Trait Self := {
     disambiguating_overlapping_traits.AgeWidget.get := get;
   }.
 End
