coq_translation/examples/traits/operator_overloading.v
@@ -80,7 +80,10 @@ Module Impl_core_ops_arith_Add_for_operator_overloading_Foo.
     Notation.dot := add;
   }.
   
-  Global Instance I : core.ops.arith.Add.Trait Self := {
+  Global Instance I :
+      core.ops.arith.Add.Trait
+        Self
+        (Rhs := (Some operator_overloading.Bar)) := {
     core.ops.arith.Add.add := add;
   }.
 End Impl_core_ops_arith_Add_for_operator_overloading_Foo.
@@ -108,7 +111,10 @@ Module Impl_core_ops_arith_Add_for_operator_overloading_Bar.
     Notation.dot := add;
   }.
   
-  Global Instance I : core.ops.arith.Add.Trait Self := {
+  Global Instance I :
+      core.ops.arith.Add.Trait
+        Self
+        (Rhs := (Some operator_overloading.Foo)) := {
     core.ops.arith.Add.add := add;
   }.
 End Impl_core_ops_arith_Add_for_operator_overloading_Bar.
